Got unify termination proved

01Unification/Unification.thy
@@ -1,20 +1,6 @@
 theory Unification
-  imports Main
+  imports "../00Utils/Utils"
 begin
-
-primrec list_sum :: "nat list \<Rightarrow> nat" where
-  "list_sum [] = 0"
-| "list_sum (n # ns) = n + list_sum ns"
-
-lemma [simp]: "length as \<noteq> length bs \<Longrightarrow> map f as \<noteq> map f bs"
-proof (induction as arbitrary: bs)
-  case Nil
-  thus ?case by (induction bs) simp_all
-next
-  case (Cons a as)
-  thus ?case by (induction bs) simp_all
-qed
-
 
 datatype expr = 
   Var string
@@ -29,9 +15,15 @@ primrec subst :: "subst \<Rightarrow> expr \<Rightarrow> expr" where
 definition extend_subst :: "string \<Rightarrow> expr \<Rightarrow> subst \<Rightarrow> subst" where
   "extend_subst x e s y = (if x = y then Some e else map_option (subst [x \<mapsto> e]) (s y))"
 
-primrec vars :: "expr \<Rightarrow> string set" where
+definition extension :: "subst \<Rightarrow> subst \<Rightarrow> bool" (infix "extends" 50) where
+  "s' extends s = (\<exists>xes. s' = fold (\<lambda>(x, e). extend_subst x e) xes s)"
+
+fun vars :: "expr \<Rightarrow> string set" 
+and varss :: "expr list \<Rightarrow> string set" where
   "vars (Var x) = {x}"
-| "vars (Ctor k es) = \<Union> (set (map vars es))"
+| "vars (Ctor k es) = varss es"
+| "varss [] = {}"
+| "varss (e # es) = vars e \<union> varss es"
 
 primrec ctors :: "expr \<Rightarrow> nat" where
   "ctors (Var x) = 0"
@@ -56,32 +48,26 @@ fun list_unifier :: "subst \<Rightarrow> (expr \<times> expr) list \<Rightarrow>
   "list_unifier s [] = True"
 | "list_unifier s ((e\<^sub>1, e\<^sub>2) # ess) = ((s unifies e\<^sub>1 and e\<^sub>2) \<and> list_unifier s ess)"
 
-function unify' :: "nat \<Rightarrow> (expr \<times> expr) list \<Rightarrow> subst \<rightharpoonup> subst" where
-  "unify' n [] s = Some s"
-| "unify' n ((Ctor k\<^sub>1 es\<^sub>1, Ctor k\<^sub>2 es\<^sub>2) # ess) s = (
-    if k\<^sub>1 = k\<^sub>2 \<and> length es\<^sub>1 = length es\<^sub>2 then unify' n (zip es\<^sub>1 es\<^sub>2 @ ess) s 
+function unify' :: "(expr \<times> expr) list \<Rightarrow> subst \<rightharpoonup> subst" where
+  "unify' [] s = Some s"
+| "unify' ((Ctor k\<^sub>1 es\<^sub>1, Ctor k\<^sub>2 es\<^sub>2) # ess) s = (
+    if k\<^sub>1 = k\<^sub>2 \<and> length es\<^sub>1 = length es\<^sub>2 then unify' (zip es\<^sub>1 es\<^sub>2 @ ess) s 
     else None)"
-| "unify' 0 ((Ctor k es, Var x) # ess) s = undefined"
-| "unify' (Suc n) ((Ctor k es, Var x) # ess) s = (
-    if x \<in> \<Union> (set (map vars es)) then None
-    else unify' n (list_subst x (Ctor k es) ess) (extend_subst x (Ctor k es) s))"
-| "unify' 0 ((Var x, Ctor k es) # ess) s = undefined"
-| "unify' (Suc n) ((Var x, Ctor k es) # ess) s = (
-    if x \<in> \<Union> (set (map vars es)) then None
-    else unify' n (list_subst x (Ctor k es) ess) (extend_subst x (Ctor k es) s))"
-| "unify' 0 ((Var x, Var y) # ess) s = (
-    if x = y \<and> x \<notin> list_vars ess then unify' 0 ess s
-    else undefined)"
-| "unify' (Suc n) ((Var x, Var y) # ess) s = (
-    if x = y then unify' (if x \<in> list_vars ess then Suc n else n) ess s
-    else unify' n (list_subst x (Var y) ess) (extend_subst x (Var y) s))"
+| "unify' ((Ctor k es, Var x) # ess) s = (
+    if x \<in> varss es then None
+    else unify' (list_subst x (Ctor k es) ess) (extend_subst x (Ctor k es) s))"
+| "unify' ((Var x, Ctor k es) # ess) s = (
+    if x \<in> varss es then None
+    else unify' (list_subst x (Ctor k es) ess) (extend_subst x (Ctor k es) s))"
+| "unify' ((Var x, Var y) # ess) s = unify' (list_subst x (Var y) ess) (extend_subst x (Var y) s)"
   by pat_completeness auto
 
 definition unify :: "expr \<Rightarrow> expr \<rightharpoonup> subst" where
-  "unify e\<^sub>1 e\<^sub>2 = unify' (card (vars e\<^sub>1 \<union> vars e\<^sub>2)) [(e\<^sub>1, e\<^sub>2)] (\<lambda>x. None)"
+  "unify e\<^sub>1 e\<^sub>2 = unify' [(e\<^sub>1, e\<^sub>2)] Map.empty"
 
 lemma [simp]: "finite (vars e)"
-  by (induction e) simp_all
+  and [simp]: "finite (varss es)"
+  by (induction e and es rule: vars_varss.induct) simp_all
 
 lemma [simp]: "finite (list_vars ess)"
   by (induction ess rule: list_vars.induct) simp_all
@@ -89,8 +75,7 @@ lemma [simp]: "finite (list_vars ess)"
 lemma [simp]: "list_vars (ess\<^sub>1 @ ess\<^sub>2) = list_vars ess\<^sub>1 \<union> list_vars ess\<^sub>2"
   by (induction ess\<^sub>1 rule: list_ctors.induct) auto
 
-lemma [simp]: "length es\<^sub>1 = length es\<^sub>2 \<Longrightarrow> 
-  list_vars (zip es\<^sub>1 es\<^sub>2) = \<Union> (vars ` set es\<^sub>1) \<union> \<Union> (vars ` set es\<^sub>2)"
+lemma [simp]: "length es\<^sub>1 = length es\<^sub>2 \<Longrightarrow> list_vars (zip es\<^sub>1 es\<^sub>2) = varss es\<^sub>1 \<union> varss es\<^sub>2"
 proof (induction es\<^sub>1 arbitrary: es\<^sub>2)
   case (Cons e\<^sub>1 es\<^sub>1)
   thus ?case by (induction es\<^sub>2) auto
@@ -106,8 +91,59 @@ proof (induction es\<^sub>1 arbitrary: es\<^sub>2)
   thus ?case by (induction es\<^sub>2) simp_all
 qed simp_all
 
+lemma [simp]: "subst [x \<mapsto> Var x] e = e"
+proof (induction e)
+  case (Ctor k es)
+  thus ?case by (induction es) simp_all
+qed simp_all
+
+lemma [simp]: "list_subst x (Var x) ess = ess"
+  by (induction x "Var x" ess rule: list_subst.induct) simp_all
+
+lemma [simp]: "x \<notin> vars e \<Longrightarrow> vars (subst [x \<mapsto> e'] e) = vars e"
+  and [simp]: "x \<notin> varss es \<Longrightarrow> varss (map (subst [x \<mapsto> e']) es) = varss es"
+  by (induction e and es rule: vars_varss.induct) simp_all
+
+lemma [simp]: "x \<in> vars e \<Longrightarrow> vars (subst [x \<mapsto> e'] e) = vars e - {x} \<union> vars e'"
+  and [simp]: "x \<in> varss es \<Longrightarrow> varss (map (subst [x \<mapsto> e']) es) = varss es - {x} \<union> vars e'"
+proof (induction e and es rule: vars_varss.induct)
+  case (4 e es)
+  hence "varss (map (subst [x \<mapsto> e']) (e # es)) = varss (e # es) - {x} \<union> vars e'" 
+    by fastforce
+  thus ?case by blast
+qed simp_all
+
+lemma [simp]: "vars (subst [x \<mapsto> e'] e) = vars e - {x} \<union> (if x \<in> vars e then vars e' else {})"
+  by simp
+
+lemma [simp]: "x \<notin> list_vars ess \<Longrightarrow> list_vars (list_subst x e ess) = list_vars ess"
+  by (induction ess rule: list_vars.induct) simp_all
+
+lemma [simp]: "x \<in> list_vars ess \<Longrightarrow> list_vars (list_subst x e ess) = list_vars ess - {x} \<union> vars e"
+proof (induction ess rule: list_vars.induct)
+  case (2 e\<^sub>1 e\<^sub>2 ess)
+  thus ?case by (cases "x \<in> list_vars ess") auto
+qed simp_all
+
+lemma [simp]: "list_vars (list_subst x e ess) = 
+    list_vars ess - {x} \<union> (if x \<in> list_vars ess then vars e else {})"
+  by simp
+
+lemma [simp]: "length (list_subst x e ess) = length ess"
+  by (induction x e ess rule: list_subst.induct) simp_all
+
+lemma [simp]: "ctors (subst [x \<mapsto> Var y] e) = ctors e"
+proof (induction e)
+  case (Ctor k es)
+  thus ?case by (induction es) simp_all
+qed simp_all
+
+lemma [simp]: "list_ctors (list_subst x (Var y) ess) = list_ctors ess"
+  by (induction x "Var y" ess rule: list_subst.induct) simp_all
+
 termination unify'
-  by (relation "measures [fst, list_ctors \<circ> fst \<circ> snd, length \<circ> fst \<circ> snd]") simp_all
+  by (relation "measures [card \<circ> list_vars \<circ> fst, list_ctors \<circ> fst, length \<circ> fst]") 
+     (simp_all add: card_insert_if)
 
 lemma [simp]: "s unifies\<^sub>l (as @ bs) = ((s unifies\<^sub>l as) \<and> (s unifies\<^sub>l bs))"
   by (induction s as rule: list_unifier.induct) simp_all
@@ -119,76 +155,33 @@ proof (induction es\<^sub>1 arbitrary: es\<^sub>2)
   thus ?case by (induction es\<^sub>2) simp_all
 qed simp_all
 
-lemma [simp]: "x \<notin> vars e \<Longrightarrow> vars (subst [x \<mapsto> e'] e) = vars e"
-  by (induction e) simp_all
-
-lemma [simp]: "x \<in> vars e \<Longrightarrow> vars (subst [x \<mapsto> e'] e) = vars e - {x} \<union> vars e'"
-proof (induction e)
-  case (Ctor k es)
-  from Ctor have "xx2a \<in> set es \<Longrightarrow> x \<in> vars xx2a \<Longrightarrow> vars (subst [x \<mapsto> e'] xx2a) = vars xx2a - {x} \<union> vars e'" by simp
-  from Ctor have "x \<in> \<Union> (set (map vars es))" by simp
-
-
-
-  have "(\<Union>xa\<in>set es. vars (subst [x \<mapsto> e'] xa)) = \<Union> (vars ` set es) - {x} \<union> vars e'" by simp
-  hence "vars (subst [x \<mapsto> e'] (Ctor k es)) = vars (Ctor k es) - {x} \<union> vars e'" by simp
-  thus ?case by blast
-qed simp_all
-
-lemma [simp]: "x \<in> list_vars ess \<Longrightarrow> list_vars (list_subst x e ess) = list_vars ess - {x} \<union> vars e"
-proof (induction ess rule: list_vars.induct)
-  case (2 e\<^sub>1 e\<^sub>2 ess)
-
-  thus ?case by simp
-qed simp_all
-
-lemma [simp]: "x \<notin> list_vars ess \<Longrightarrow> list_vars (list_subst x e ess) = list_vars ess"
-  by (induction ess rule: list_vars.induct) simp_all
-
-lemma unify_none [simp]: "unify' (card (list_vars ess)) ess s = None \<Longrightarrow> \<nexists>s'. s' unifies\<^sub>l ess"
-proof (induction "card (list_vars ess)" ess s rule: unify'.induct)
+lemma unify_none [simp]: "unify' ess s = None \<Longrightarrow> \<nexists>s'. s' extends s \<and> s' unifies\<^sub>l ess"
+proof (induction ess s rule: unify'.induct)
   case (2 k\<^sub>1 es\<^sub>1 k\<^sub>2 es\<^sub>2 ess s)
   thus ?case by (cases "k\<^sub>1 = k\<^sub>2 \<and> length es\<^sub>1 = length es\<^sub>2") simp_all
 next
-  case (4 k es x ess s)
+  case (3 k es x ess s)
   thus ?case by simp
 next
-  case (6 n x k es ess s)
+  case (4 x k es ess s)
   thus ?case by simp
 next
-  case (8 n x y ess s)
-  thus ?case
-  proof (cases "x = y")
-    case True note T = True
-    with 8 show ?thesis 
-    proof (cases "x \<in> list_vars ess")
-      case True
-      from 8 T have X: "card (insert x (list_vars ess)) = Suc n" by simp
-      with 8 T True have "unify' (Suc n) ess s = None" by fastforce
-      with 8 T True X show ?thesis by (simp add: insert_absorb)
-    qed simp_all
-  next
-    case False
-    from 8 False have "n = card (list_vars (list_subst [x \<mapsto> Var y] ess)) \<Longrightarrow>
-      unify' (card (list_vars (list_subst [x \<mapsto> Var y] ess))) (list_subst [x \<mapsto> Var y] ess) (extend_subst x (Var y) s) =
-      None \<Longrightarrow>
-      \<nexists>s'. s' unifies\<^sub>l list_subst [x \<mapsto> Var y] ess" by simp
-    from 8 have "card (insert y (insert x (list_vars ess))) = Suc n" by simp
-    with 8 False have "unify' n (list_subst [x \<mapsto> Var y] ess) (extend_subst x (Var y) s) = None" by simp
+  case (5 x y ess s)
+  from 5 have "\<nexists>s'. s' unifies\<^sub>l list_subst x (Var y) ess" by simp
+  from 5 have "unify' (list_subst x (Var y) ess) (extend_subst x (Var y) s) = None" by simp
 
 
-
-    have "\<And>s'. (case s' x of None \<Rightarrow> Var x | Some e \<Rightarrow> e) = (case s' y of None \<Rightarrow> Var y | Some e \<Rightarrow> e)
-       \<Longrightarrow> \<not> s' unifies\<^sub>l ess" by simp
-    thus ?thesis by simp
-  qed
+  have "\<forall>s'. (case s' x of None \<Rightarrow> Var x | Some e \<Rightarrow> e) = (case s' y of None \<Rightarrow> Var y | Some e \<Rightarrow> e) \<longrightarrow> \<not> s' unifies\<^sub>l ess" by simp
+  thus ?case by simp
 qed simp_all
+
+lemma [simp]: "s extends Map.empty"
+  by (unfold extension_def)
 
 lemma [simp]: "unify e\<^sub>1 e\<^sub>2 = None \<Longrightarrow> \<nexists>s. s unifies e\<^sub>1 and e\<^sub>2"
 proof (unfold unify_def)
-  assume "unify' (card (vars e\<^sub>1 \<union> vars e\<^sub>2)) [(e\<^sub>1, e\<^sub>2)] (\<lambda>x. None) = None"
-  hence "unify' (card (list_vars [(e\<^sub>1, e\<^sub>2)])) [(e\<^sub>1, e\<^sub>2)] (\<lambda>x. None) = None" by simp
-  hence "\<nexists>s'. s' unifies\<^sub>l [(e\<^sub>1, e\<^sub>2)]" by (metis unify_none)
+  assume "unify' [(e\<^sub>1, e\<^sub>2)] Map.empty = None"
+  hence "\<nexists>s'. s' extends Map.empty \<and> s' unifies\<^sub>l [(e\<^sub>1, e\<^sub>2)]" by (metis unify_none)
   thus "\<nexists>s. s unifies e\<^sub>1 and e\<^sub>2" by simp
 qed
 
